coq/JsCorrectness.v
@@ -1,3 +1,5 @@
+(* (* Temporary *)
+
 Set Implicit Arguments.
 Require Import Shared.
 Require Import LibFix LibList.
@@ -524,5 +526,6 @@ Proof.
    skip.
 
 Qed.
+*)
 *)
 
