coq/JsInterpreterExtraction.v
@@ -207,14 +207,14 @@ Extract Constant parse_pickable => "(fun s ->
 
 
 (* Debugging *)
-Extract Constant stuck_because => "(fun s ->
+Extract Constant impossible_because => "(fun s ->
   print_endline (""Stuck because:\t"" ^ Prheap.string_of_char_list s) ;
   Coq_result_stuck)".
-Extract Constant stuck_heap => "(fun s message ->
+Extract Constant impossible_with_heap_because => "(fun s message ->
   print_endline (""Stuck!\nState: "" ^ Prheap.prstate true s
     ^ ""\nMessage:\t"" ^ Prheap.string_of_char_list message) ;
   Coq_result_stuck)".
-Extract Constant stuck_because_other => "(fun s ->
+Extract Constant impossible_because_other => "(fun s ->
   print_endline (""Stuck because:\t"" ^ Prheap.string_of_char_list s) ;
   raise Not_found)".
 
